commit9

proiectPLP.v
@@ -418,10 +418,13 @@ Check envMem.
 Compute (update_mem mem envMem "sal" mem_default default).
 Compute (update_mem mem ( update_env envMem  "x" (offset 5)) "x" mem_default (naturals (num 5))).
 
+
 Definition update_list_globale ( l : list Var ) ( x : Var )
     : list Var := l++ [x].
+Definition update_list_locale ( l : list Var ) ( x : Var )
+    : list Var := l++ [x].
 Definition update_list_functii ( l : list Var ) ( x : Var )  
-    : list Var := l++  [x].
+    : list Var := l++ [x].
 Fixpoint search_functie ( l:list Var ) (x : Var) : eroareBool :=
   match l with
   | [] => boolean false
@@ -433,6 +436,8 @@ Compute search_functie ["a" ; "b" ; "c" ] "c".
 Compute update_list_globale ["a";"b"] "c". 
 Definition parametrii1 := Parametrii.
 Definition parametrii2 := Parametrii.
+
+
 
 Reserved Notation "S -{ Sigma }-> Sigma'" (at level 60).
 Inductive eval : Stmt -> Env -> Env -> Prop :=
@@ -488,16 +493,101 @@ Inductive eval : Stmt -> Env -> Env -> Prop :=
     (lambda x parametrii1 parametrii2 s) -{ sigma1 }-> sigma2
 | e_apelare : forall x b lista parametrii1 sigma1 sigma2,
     b = search_functie lista x ->
-    b = true ->
+    (* b = true -> *)
     (apelare_functie x parametrii1) -{ sigma1 }-> sigma2
 | e_coments : forall s sigma1 sigma2 ,
     /* s *\ -{ sigma1 }-> sigma2 
 where "s -{ sigma }-> sigma'" := (eval s sigma sigma').
 
-Definition update_functie ( s : Stmt) ( env env' : Env ) : Prop :=
-  match s with
-  | _ => (eval s env env')
+(* Inductive Instruction :=
+| push_stmt : Stmt -> Instruction.
+Inductive run_Instruction :=
+| compil_stmt : Stmt -> run_Instruction.
+Definition Stackf := list Stmt.
+Definition add_instruction (i : Instruction) (stack : Stackf) : Stackf :=
+  match i with
+  | push_stmt c => (c :: stack)
+  end.
+Definition compil_Instruction (i : run_Instruction) (env env1 :Env)  : Prop :=
+  match i with
+  | compil_stmt s => ( s -{ env }-> env1)
+end. 
+Definition compile (e : Stmt) : list Instruction :=
+  match e with
+  | nat_decl a => []
+  | nat_assign a x => []
+  | nat_decl_assign a x=> []
+  | bool_decl a => []
+  | bool_assign a x=> []
+  | bool_decl_assign a x=> []
+  | apelare_functie x c => []
+  | sequence a b => [push_stmt a]
+  | while b c=> [push_stmt c]
+  | ifthen b c => [push_stmt c]
+  | ifelse b a c => [push_stmt c]
+  | lambda x a b c => [push_stmt c]
+  | comentarii c => [push_stmt c]
 end.
+Reserved Notation "S -f{ Sigma }f-> Sigma'" (at level 60).
+Inductive eval_functii : Stmt -> Env -> Env -> Prop :=
+| e_nat_assign1: forall a i x sigma sigma',
+   a =[ sigma ]=> i ->
+   sigma' = (update sigma x (naturals i)) ->
+   (nat_assign x a) -f{ sigma }f-> sigma'
+| e_nat_decl1: forall x sigma sigma',
+    sigma' = (update sigma x err_assign) ->
+    (nat_decl x) -f{ sigma }f-> sigma'
+| e_nat_decl_assign1: forall a i x sigma sigma',
+   a =[ sigma ]=> i ->
+   sigma' = (update sigma x (naturals i)) ->
+   (nat_decl_assign x a) -f{ sigma }f-> sigma'
+
+| e_bool_decl1: forall x sigma sigma',
+   sigma' = (update sigma x err_undecl) ->
+   (bool_decl x) -f{ sigma }f-> sigma'
+| e_bool_assign1: forall a i x sigma sigma',
+    a ={ sigma }=> i ->
+    sigma' = (update sigma x (booleans i)) ->
+    (bool_assign x a) -f{ sigma }f-> sigma'
+| e_bool_decl_assign1: forall a i x sigma sigma',
+    a ={ sigma }=> i ->
+    sigma' = (update sigma x (booleans i)) ->
+    (bool_decl_assign x a) -f{ sigma }f-> sigma'
+
+| e_seq1 : forall s1 s2 sigma sigma1 sigma2,
+    s1 -{ sigma }-> sigma1 ->
+    s2 -{ sigma1 }-> sigma2 ->
+    (s1 ;; s2) -f{ sigma }f-> sigma2
+| e_if_then1 : forall b s sigma sigma',
+    b ={ sigma }=> true ->
+    s -{ sigma }-> sigma' ->
+    ifthen b s -f{ sigma }f-> sigma
+| e_if_then_elsetrue1 : forall b s1 s2 sigma sigma',
+    b ={ sigma }=>true ->
+    s1 -{ sigma }-> sigma' ->
+    ifelse b s1 s2 -f{ sigma }f-> sigma' 
+| e_if_then_elsefalse1 : forall b s1 s2 sigma sigma',
+    b ={ sigma }=> boolean false ->
+    s2 -{ sigma }-> sigma' ->
+    ifelse b s1 s2 -f{ sigma }f-> sigma' 
+| e_whilefalse1 : forall b s sigma,
+    b ={ sigma }=> false ->
+    while b s -f{ sigma }f-> sigma
+| e_whiletrue1 : forall b s sigma sigma',
+    b ={ sigma }=>  true ->
+    (s ;; while b s) -f{ sigma }f-> sigma' ->
+    while b s -f{ sigma }f-> sigma'
+| e_lambda1 : forall x s parametrii1 parametrii2 sigma1 sigma2,
+    s -{ sigma1 }-> sigma2 ->
+    (lambda x parametrii1 parametrii2 s) -f{ sigma1 }f-> sigma2
+| e_apelare1 : forall x b lista parametrii1 stack sigma1 sigma2,
+    b = search_functie lista x ->
+     compil_Instruction stack sigma1 sigma2 ->
+    (apelare_functie x parametrii1) -f{ sigma1 }f-> sigma2
+| e_coments1 : forall s sigma1 sigma2 ,
+    /* s *\ -f{ sigma1 }f-> sigma2 
+where "s -f{ sigma }f-> sigma'" := (eval_functii s sigma sigma').
+ *)
 
 Reserved Notation "S -*{ Sigma }*-> Sigma'" (at level 60).
 Inductive evalprograms : Programs -> Env -> Env -> Prop :=
@@ -505,8 +595,9 @@ Inductive evalprograms : Programs -> Env -> Env -> Prop :=
     sigma' = (update sigma x (naturals (num 0))) ->
     list_glb' = (update_list_globale list_glb x) ->
     (decl_var_globale x) -*{ sigma }*-> sigma'
-| e_decl_functie: forall x s Parametrii y list_functii list_functii' sigma sigma',
-    s -{ sigma }-> sigma' ->
+| e_decl_functie: forall x s Parametrii  y list_functii list_functii' sigma sigma',
+    s -{ sigma }-> sigma' -> 
+    (* stack2= compile s -> *)
     list_functii' = ( update_list_functii list_functii x)->
     (decl_functie x Parametrii s y) -*{ sigma }*-> sigma'
 | e_decl_functie_main : forall s sigma sigma',
@@ -605,64 +696,50 @@ Definition max1 :=
   decl_functie_main ( (int "a") ;;
                        ("a" :n=3 );;
                        lambda "lbd" [] [] ("a":n="a"-'1);;  
-                      Do { 
-                          "a":n="a"-'1
-                       }while* ( "a" <=' 0);;
+                      
                        apelare_functie "da" [ "a";"b" ]
                        ).
 
 Definition state0 := fun (x:Var) => err_undecl.
 Example eval_max1 : 
- exists state, max1 -*{ state0 }*-> state /\ state "a" = naturals (num 2).
+ exists state, max1 -*{ state0 }*-> state .
 Proof.
   eexists.
-  split.
   - unfold max1. 
     eapply e_seq_prg.
     ++ eapply e_seq_prg.
         +++ eapply e_decl_global;eauto.
-        +++ eapply e_decl_functie; eauto. eapply e_seq. 
-            ++++ eapply e_nat_assign.
-                +++++ eapply const.
-                +++++ split.
-            ++++ eapply e_nat_assign.
-                +++++ eapply substract.
-                 -- eapply var.
-                 -- eapply const.
-                 -- split.
-                +++++ split.
-   ++ eapply e_seq_prg.
+        +++ eapply e_decl_functie; eauto.
+          ++++ eapply e_seq.
+            +++++ eapply e_nat_assign.
+              ++++++ eapply const.
+              ++++++ split.
+             +++++ eapply e_nat_assign.
+              ++++++ eapply substract.
+                -- eapply var.
+                -- eapply const.
+                -- split.
+              ++++++ split.
+    ++ eapply e_seq_prg.
       +++ simpl. eapply e_decl_global; eauto.
       +++ eapply e_decl_functie_main. 
           eapply e_seq.
           ++++ eapply e_seq.
             +++++ eapply e_seq.
-              ++++++eapply e_seq.
               +++++++ eapply e_nat_decl.
                 ++++++++ simpl. split. 
               +++++++ eapply e_nat_assign.
                     ---- eapply const.
                     ---- split.
-             ++++++ eapply e_lambda. eapply e_nat_assign.
+             +++++ eapply e_lambda. eapply e_nat_assign.
                    +++++++ eapply substract.
                     ++++++++ eapply var.
                     ++++++++ eapply const.
                     ++++++++ split.
                    +++++++ split.
-             +++++ eapply e_seq.
-                ++++++ eapply e_nat_assign.
-                    +++++++ eapply substract.
-                      ++++++++ eapply var. 
-                      ++++++++ eapply const.
-                      ++++++++ split.
+             ++++ eapply e_apelare.
                     +++++++ split.
-               ++++++ eapply e_whilefalse.
-                    +++++++ eapply b_lessthan.
-                    +++++++++ eapply var.
-                    +++++++++ eapply const.
-                    +++++++++ simpl. reflexivity.
-              ++++ eapply e_apelare. eauto. 
-               +++++  Abort.
+Abort.
 
 Inductive string  :=
   | EmptyString : string
